Congruences for WBisim

sme/Sme/ITree/WBisim.lean
@@ -1,13 +1,19 @@
 import CoinductivePredicates
 import Sme.ITree.Defs
 import Sme.ITree.Combinators
+import Sme.ITree.KTree
 
-namespace Sme.ITree
+namespace Sme
 
 universe u v
 
 variable {E : Type u → Type u} {A B C : Type (u + 1)}
 
+namespace ITree
+
+/-- Given Some sequence of taus, they are related to the first productive value
+  Step (tau (tau (r))) r
+-/
 inductive Step : Base E (ITree E A) A → Base E (ITree E A) A → Type _
   | tau {a b} : Step a.dest b → Step (.tau a) b
   | ret {v} : Step (.ret v) (.ret v)
@@ -78,9 +84,14 @@ theorem no_middle (V : Base E _ A)
 
 end Step
 
+/-- EStep (tau (tau (r))) (tau r) -/
 inductive EStep : Base E (ITree E A) A → Base E (ITree E A) A → Type _
   | tau {a b} : EStep a.dest b → EStep (.tau a) b
   | refl a : EStep a a
+
+def Step.toEStep {a b : Base E _ A} : Step a b → EStep a b
+  | .vis | .ret => .refl _
+  | .tau h => .tau (toEStep h)
 
 namespace EStep
 
@@ -95,15 +106,106 @@ def step_comp {a b c : Base E _ A} : EStep a b → Step b c → Step a c
   | .refl _, v => v
   | .tau h, ha => .tau (step_comp h ha)
 
-theorem spin {a} (h : EStep a ((spin : ITree E A).dest)) : a = spin.dest := by
-  generalize h' : ITree.dest ITree.spin = v at h
+theorem spinEq {a} (h : EStep a (.tau (spin : ITree E A))) : a = .tau spin := by
+  generalize h' : Base.tau (spin : ITree E A) = v at h
   induction h
   case tau h =>
     subst h'
     specialize h rfl
+    rw [←spin.dest_eq] at h
     obtain rfl := dest.inj_eq.mp h
     simp
   · rfl
+
+theorem eqSpin {a} (h : EStep (.tau (spin : ITree E A)) a) : a = .tau spin := by
+  generalize h' : Base.tau (spin : ITree E A) = v at h
+  induction h
+  case tau ih =>
+    obtain rfl := Base.tau.inj h'
+    rw [spin.dest_eq] at ih
+    exact ih rfl
+  · rfl
+
+def middle : {a c d : Base E _ A} → EStep a c → EStep a d → (EStep d c ⊕ EStep c d)
+  | _, _, _, .refl _, h => .inr h
+  | _, _, _, .tau h', .refl _ => .inl <| .tau h'
+  | _, _, _, .tau h', .tau h => middle h' h
+
+def meet {a b c : Base E _ A} : EStep a b → Step a c → Step b c
+  | .tau h, .tau h' => meet h h'
+  | .refl _, v => v
+
+def triag {a b c d : Base E _ A} : EStep a c → EStep b c → Step a d → Step b d
+  | .refl _, h, h' => h.step_comp h'
+  | .tau ha, .tau hb, .tau h' =>
+    .tau (triag ha hb h')
+  | .tau ha, .refl _, .tau hb => meet ha hb
+
+def max {a b c : Base E _ A} : EStep a b → EStep a c → Base E (ITree E A) A
+  | .refl _, _ => c
+  | _, .refl _ => b
+  | .tau ha, .tau hb => max ha hb
+
+theorem max_comm {a b c : Base E _ A} : (x : EStep a b) → (y : EStep a c) → max x y = max y x
+  | .refl _, .refl _ | .tau _, .refl _ | .refl _, .tau _ => rfl
+  | .tau x, .tau y => max_comm x y
+
+@[simp]
+theorem max_toEStep_l {a b c : Base E _ A} : {x : EStep a b} → {y : Step a c} → max x y.toEStep = c
+  | .refl _, _ => by simp only [max]
+  | .tau a, .tau b => by 
+    simp [max, Step.toEStep]
+    apply max_toEStep_l
+
+@[simp]
+theorem max_toEStep_r
+    {a b c : Base E _ A} {x : EStep a b} {y : Step a c} : max y.toEStep x = c := by
+  rw [max_comm, max_toEStep_l]
+
+def maxl {a b c : Base E _ A} : (x : EStep a b) → (y : EStep a c) → EStep b (max x y)
+  | .refl _, .refl _ => .refl _
+  | .refl _, .tau v => .tau v
+  | .tau v, .refl _ => .refl _
+  | .tau ha, .tau hb => maxl ha hb
+
+def maxr {a b c : Base E _ A} : (x : EStep a b) → (y : EStep a c) → EStep c (max x y)
+  | .refl _, .refl _ => .refl _
+  | .refl _, .tau v => .refl _
+  | .tau v, .refl _ => .tau v
+  | .tau ha, .tau hb => maxr ha hb
+
+@[simp]
+def ret {w v} : EStep (.ret w) (v : Base E _ A) → v = .ret w
+  | .refl _ => rfl
+
+@[simp]
+def vis {X e k v} : EStep (.vis (e : E X) k) (v : Base E _ A) → v = .vis e k
+  | .refl _ => rfl
+
+theorem toRetStep {v} {a : Base E _ A}
+    (h : EStep a (.ret v)) : Nonempty (Step a (.ret v)) := by 
+  rcases Step.no_middle a with (rfl|⟨w,⟨p⟩⟩|⟨_,_,_,⟨p⟩⟩)
+  · have := EStep.eqSpin h
+    contradiction
+  · cases meet h p
+    exact ⟨p⟩
+  · cases meet h p
+
+theorem toVisStep {X e k} {a : Base E _ A}
+    (h : EStep a (.vis (e : E X) k)) : Nonempty (Step a (.vis e k)) := by 
+  rcases Step.no_middle a with (rfl|⟨w,⟨p⟩⟩|⟨_,_,_,⟨p⟩⟩)
+  · have := EStep.eqSpin h
+    contradiction
+  · cases meet h p
+  · cases meet h p
+    exact ⟨p⟩
+
+def transp_bind_map
+    (f : A → ITree E B) {a b : Base E _ A}
+    : EStep a b
+    → EStep (bind_map f a) (bind_map f b)
+  | .tau h => .tau <| dest_bind ▸ transp_bind_map f h
+  | .refl _ => .refl _
 
 end EStep
 
@@ -112,7 +214,7 @@ coinductive WBisim' (E : Type u → Type u) (A : Type (u + 1))
   -- This case only exists for refl spin spin,
   -- in fact it could be this,
   -- but that would be harder to prove things about
-  | refl {a} : WBisim' E A a a
+  | refl {a b c} : EStep a c → EStep b c → WBisim' E A a b
   | ret {a b v}
       : Step a (.ret v) → Step b (.ret v) → WBisim' E A a b
   | vis {V e a b a' b'}
@@ -121,15 +223,90 @@ coinductive WBisim' (E : Type u → Type u) (A : Type (u + 1))
 
 namespace WBisim'
 
+namespace Invariant
+
+theorem eqSpin {R b}
+    (v : Invariant E A R (Base.tau spin) b)
+    : Base.tau spin = b := by
+  rcases v with (⟨h, h'⟩|h|h)
+  · obtain rfl := h.eqSpin
+    obtain rfl := h'.spinEq
+    rfl
+  · exact h.not_spin'.elim
+  · exact h.not_spin'.elim
+
+theorem ofEstep {R c d}
+    (v' : EStep d c)
+    : Invariant E A R c d := by
+  refine .refl (.refl _) v'
+
+theorem antisymm {R}
+    {a b : Base E _ A}
+    (hab : EStep a b) (hba : EStep b a)
+    : Invariant E A R a b := by
+  rcases Step.no_middle a with (rfl|⟨_,⟨h⟩⟩|⟨_,_,_,⟨h⟩⟩)
+  · obtain rfl := hab.eqSpin
+    exact .refl (.refl _) (.refl _)
+  · exact .ret h (EStep.step_comp hba h)
+  · refine .refl h.toEStep (EStep.step_comp hba h).toEStep
+
+-- TODO: Clean...
+theorem skip
+    {R : _ → _ → Prop} {a b c d}
+    (ha : EStep a c) (ha : EStep b d)
+    (v : WBisim'.Invariant E A R c d)
+    : WBisim'.Invariant E A R a b := by
+  rcases Step.no_middle c with (rfl|⟨_,⟨r⟩⟩|⟨_,_,_,⟨r⟩⟩)
+  · obtain rfl:= ha.spinEq
+    obtain rfl := v.eqSpin
+    obtain rfl:= ha.spinEq
+    exact .refl (.refl _) (.refl _)
+  · rename_i ha' _
+    rcases v with (⟨v', v⟩|⟨v', v⟩|⟨v', v, h⟩)
+    · exact .refl (ha'.trans v') (ha.trans v)
+    · refine .ret (ha'.step_comp v') (ha.step_comp v)
+    · refine .vis (ha'.step_comp v') (ha.step_comp v) h
+  · rename_i ha' _ _ _
+    rcases v with (⟨v', v⟩|⟨v', v⟩|⟨v', v, h⟩)
+    · exact .refl (ha'.trans v') (ha.trans v)
+    · refine .ret (ha'.step_comp v') (ha.step_comp v)
+    · refine .vis (ha'.step_comp v') (ha.step_comp v) h
+
+theorem refl'
+    {R a}
+    : WBisim'.Invariant E A R a a := 
+  .refl (.refl _) (.refl _)
+
+theorem shrink
+    {R : _ → _ → Prop} {a b c d}
+    (ha : EStep a c) (hb : EStep b d)
+    (v : WBisim'.Invariant E A R a b)
+    : WBisim'.Invariant E A R c d := by
+  rcases v with (⟨x, y⟩|⟨x, y⟩|⟨x,y,h⟩)
+  · exact refl
+      (c := (x.maxl ha).max (y.maxl hb))
+      ((x.maxr ha).trans (EStep.maxl _ _))
+      ((y.maxr hb).trans (EStep.maxr _ _))
+  · have ha := ha.maxl x.toEStep
+    have hb := hb.maxl y.toEStep
+    simp at ha hb
+    exact .ret (Classical.choice ha.toRetStep) (Classical.choice hb.toRetStep)
+  · have ha := ha.maxl x.toEStep
+    have hb := hb.maxl y.toEStep
+    simp at ha hb
+    exact .vis (Classical.choice ha.toVisStep) (Classical.choice hb.toVisStep) h
+
+end Invariant
+
 theorem unfold : Is E A (WBisim' E A) :=
   fun ⟨r, ris, rab⟩ =>
     match ris rab with
-    | .refl => .refl
+    | .refl ha hb => .refl ha hb
     | .ret a b => .ret a b
     | .vis a b h => .vis a b fun v => ⟨r, ris, h v⟩
 
 @[refl]
-theorem refl {a} : WBisim' E A a a := ⟨(· = ·), fun v => v ▸ .refl, rfl⟩
+theorem refl {a} : WBisim' E A a a := ⟨(· = ·), fun v => v ▸ .refl (.refl _) (.refl _), rfl⟩
 
 theorem ret {a b v} (ha : Step a (.ret v)) (hb : Step b (.ret v))
     : WBisim' E A a b := ⟨
@@ -146,12 +323,36 @@ theorem vis {V e a b a' b'}
   fun
     | .inl v =>
       match v.unfold with
-      | .refl => .refl
+      | .refl ha hb => .refl ha hb
       | .ret a b => .ret a b
       | .vis a b h => .vis a b fun _ => .inl <| h _
     | .inr ⟨a, b⟩ => .vis a b fun _ => .inl <| h _,
   .inr ⟨ha, hb⟩
 ⟩
+
+theorem eqSpin {a} (h : WBisim' E A a spin.dest) : a = spin.dest :=
+  match h.unfold with
+  | .refl ha hb => by
+    obtain rfl := (spin.dest_eq ▸ hb).eqSpin
+    obtain rfl := ha.spinEq
+    rw [spin.dest_eq]
+  | .ret _ v => (Step.not_spin v).elim
+  | .vis _ v _ => (Step.not_spin v).elim
+
+theorem eqSpin' {a} (h : WBisim' E A a (.tau spin)) : a = (.tau spin) := by
+  rw [←spin.dest_eq] at h ⊢
+  exact eqSpin h
+
+theorem symm {a b} : WBisim' E A a b → WBisim' E A b a :=
+  fun ⟨r, ris, rab⟩ => ⟨
+    fun a b => r b a,
+    fun rab =>
+      match ris rab with
+      | .ret a b => .ret b a
+      | .refl ha hb => .refl hb ha
+      | .vis a b h => .vis b a h,
+    rab,
+  ⟩
 
 @[elab_as_elim]
 theorem cases {a b} {motive : Base E _ A → Base E _ A → Prop}
@@ -164,43 +365,39 @@ theorem cases {a b} {motive : Base E _ A → Base E _ A → Prop}
       → (∀ v : V, WBisim' E A (f v).dest (g v).dest) → motive a b)
     : motive a b :=
   match h.unfold with
-  | .refl => by
+  | .refl ha hb => by
+    /- have :=  -/
     rcases Step.no_middle a with (rfl|⟨_, ⟨p⟩⟩|⟨_,_,f,⟨p⟩⟩)
-    · exact hRefl
-    · exact hRet p p
-    · apply hVis p p fun _ => .refl
+    · obtain rfl:= h.symm.eqSpin'
+      exact hRefl
+    · apply hRet p (EStep.triag ha hb p)
+    · apply hVis p (EStep.triag ha hb p) fun _ => .refl
   | .ret a b => hRet a b
   | .vis a b h => hVis a b h
-
-theorem symm {a b} : WBisim' E A a b → WBisim' E A b a :=
-  fun ⟨r, ris, rab⟩ => ⟨
-    fun a b => r b a,
-    fun rab =>
-      match ris rab with
-      | .ret a b => .ret b a
-      | .refl => .refl
-      | .vis a b h => .vis b a h,
-    rab,
-  ⟩
 
 theorem trans {a b c} : WBisim' E A a b → WBisim' E A b c → WBisim' E A a c :=
   fun ⟨r, ris, rab⟩ ⟨r', ris', rbc⟩ => ⟨
     (fun a c => r a c ∨ r' a c ∨ ∃ b, r a b ∧ r' b c),
     fun
       | .inl v  => (match ris v with
-        | .refl => .refl
+        | .refl ha hb => .refl ha hb
         | .ret a b => .ret a b
         | .vis a b h => .vis a b fun v => .inl (h v))
       | .inr <| .inl v  => (match ris' v with
-        | .refl => .refl
+        | .refl ha hb => .refl ha hb
         | .ret a b => .ret a b
         | .vis a b h => .vis a b fun v => .inr <| .inl (h v))
       | .inr <| .inr ⟨_, rab, rbc⟩ => (match ris rab, ris' rbc with
-        | .refl, .refl => .refl
-        | .ret a b, .refl
-        | .refl, .ret a b => .ret a b
-        | .vis a b h, .refl => .vis a b (fun x => .inl <| h x)
-        | .refl, .vis a b h => .vis a b (fun x => .inr <| .inl <| h x)
+        | .refl ha hb, .refl ha' hb' =>
+          .skip ha hb' (.shrink hb ha' .refl')
+        | .ret a b, .refl ha hb =>
+          .skip (.refl _) hb <| .shrink (.refl _) ha <| .ret a b
+        | .refl ha hb, .ret a b =>
+          .skip ha (.refl _) <| .shrink hb (.refl _) <| .ret a b
+        | .vis a b h, .refl ha hb =>
+          .skip (.refl _) hb <| .shrink (.refl _) ha <| .vis a b (fun x => .inl <| h x)
+        | .refl ha hb, .vis a b h =>
+          .skip ha (.refl _) <| .shrink hb (.refl _) <| .vis a b (fun x => .inr <| .inl <| h x)
         | .vis a b h, .vis b' a' h' => by
           obtain ⟨rfl, rfl, rfl⟩ := (Base.vis.injEq _ _ _ _ _).mp <| b.eq b'
           exact .vis a a' (fun v => .inr <| .inr <| ⟨_, h v, h' v⟩)
@@ -214,20 +411,12 @@ theorem trans {a b c} : WBisim' E A a b → WBisim' E A b c → WBisim' E A a c 
     .inr <| .inr ⟨_, rab, rbc⟩,
   ⟩
 
-theorem eqSpin {a} (h : WBisim' E A a spin.dest) : a = spin.dest :=
-  h.cases rfl (fun _ h => (Step.not_spin h).elim) (fun _ h => (Step.not_spin h).elim)
-
-theorem eqSpin' {a} (h : WBisim' E A a (.tau spin)) : a = (.tau spin) :=
-  h.cases rfl (fun _ h => (Step.not_spin' h).elim) (fun _ h => (Step.not_spin' h).elim)
-
 theorem tau {a} : WBisim' E A (Base.tau a) a.dest := ⟨
   (fun a b => Nonempty (EStep a b)),
   fun {a b} ⟨ha⟩ => by
     rcases Step.no_middle b with (rfl|⟨_, ⟨h⟩⟩|⟨_,_,_, ⟨h⟩⟩)
-    · rw [←spin.dest_eq] at ha
-      obtain rfl := ha.spin
-      rw [spin.dest_eq]
-      exact .refl
+    · obtain rfl := ha.spinEq
+      exact .refl (.refl _) (.refl _)
     · refine .ret ?_ h
       exact ha.step_comp h
     · refine .vis (ha.step_comp h) h fun _ => ⟨.refl _⟩
@@ -235,7 +424,7 @@ theorem tau {a} : WBisim' E A (Base.tau a) a.dest := ⟨
   ⟨.tau <| .refl _⟩
 ⟩
 
-theorem ofEStep {a b} : EStep a b → WBisim' E A a b 
+theorem ofEStep {a b} : EStep a b → WBisim' E A a b
   | .tau h => .trans tau (ofEStep h)
   | .refl _ => .refl
 
@@ -244,7 +433,11 @@ end WBisim'
 def WBisim {E : Type u → Type u} {A : Type (u + 1)} (a b : ITree E A) : Prop :=
   WBisim' E A a.dest b.dest
 
-infix:100 " ≈ " => WBisim
+end ITree
+
+infix:100 " ≈ " => ITree.WBisim
+
+namespace ITree
 
 namespace WBisim
 
@@ -283,7 +476,149 @@ theorem tau : .tau a ≈ a := by
 theorem tau_bind {f : _ → ITree E B} {a : ITree E A} : bind (.tau a) f ≈ bind a f :=
   ITree.tau_bind ▸ tau
 
-end WBisim
+theorem ret {v} (ha : Step a.dest (.ret v)) (hb : Step b.dest (.ret v))
+    : a ≈ b := WBisim'.ret ha hb
 
-end Sme.ITree
+theorem vis {V e a' b'}
+      (ha : Step a.dest (.vis e a')) (hb : Step b.dest (.vis e b'))
+      (h : ∀ v : V, (a' v) ≈ (b' v))
+      : a ≈ b := WBisim'.vis ha hb h
+
+instance : Trans (· ≈ · : ITree E A → _ → Prop) (· ≈ ·) (· ≈ ·) where
+  trans := trans
+
+end ITree.WBisim
+
+namespace KTree
+
+open scoped ITree
+
+def WBisim {A B} : KTree E A B → KTree E A B → Prop :=
+  fun a b => ∀ v, a v ≈ b v
+
+end KTree
+
+scoped infix:100 " ≈ₖ " => KTree.WBisim
+
+namespace ITree.WBisim'
+def stepRet {a b c} : Step a (.ret c) → WBisim' E A a b → Nonempty (Step b (.ret c)) :=
+  fun he hb =>
+  have := hb.symm.trans <| ofEStep he.toEStep
+  by
+  rcases this.unfold with (⟨ha, hb⟩|⟨h',(_|_)⟩|⟨_,(_|_),_⟩)
+  · obtain rfl := hb.ret
+    exact ha.toRetStep
+  · exact ⟨h'⟩
+
+theorem stepVis {X} {a b e k}
+    : Step a (.vis (e : E X) k) → WBisim' E A a b → ∃ k', k' ≈ₖ k ∧ Nonempty (Step b (.vis e k')) :=
+  fun he hb =>
+  have := hb.symm.trans <| ofEStep he.toEStep
+  by
+  rcases this.unfold with (⟨ha, hb⟩|⟨h',(_|_)⟩|⟨_,(_|_),_⟩)
+  · obtain rfl := hb.vis
+    exact ⟨_, fun _ => .refl, ha.toVisStep⟩
+  · rename_i h a
+    exact ⟨_, a, ⟨h⟩⟩
+
+end ITree.WBisim'
+
+namespace ITree.WBisim
+
+variable {A B : Type (u + 1)} {X : Type u}
+
+variable {a b : ITree E A}
+
+theorem tau_congr
+    (h : a ≈ b)
+    : ITree.tau a ≈ ITree.tau b := calc
+  a.tau
+    ≈ a     := tau
+  _ ≈ b     := h
+  _ ≈ b.tau := tau.symm
+
+theorem vis_congr {e : E X} {k1 k2 : KTree E X A} (h : k1 ≈ₖ k2)
+    : ITree.vis e k1 ≈ .vis e k2 :=
+  vis (e := e) (dest_vis ▸ Step.vis) (dest_vis ▸ Step.vis) h
+
+theorem bind_congr_arg
+    {X} {k1 : KTree E A X}
+    (h : a ≈ b)
+    : bind a k1 ≈ bind b k1 := by
+  simp [WBisim]
+  refine ⟨
+    fun a b => ∃ c d , WBisim' E A c d
+        ∧ bind_map k1 c = a
+        ∧ bind_map k1 d = b,
+    ?_,
+    ⟨_,_, h, rfl, rfl⟩
+  ⟩
+  rintro a b (⟨x, y, h, rfl, rfl⟩)
+  rcases Step.no_middle y with (rfl|⟨⟨_,⟨h'⟩⟩⟩|⟨⟨_,_,_,⟨h'⟩⟩⟩)
+  · obtain rfl := h.eqSpin'
+    exact .refl (.refl _) (.refl _)
+  · have ⟨h⟩ := WBisim'.stepRet h' h.symm
+    have h := h.toEStep.transp_bind_map k1
+    have h' := h'.toEStep.transp_bind_map k1
+    simp at h h'
+    exact .refl h h'
+  · have ⟨_, bs, ⟨h⟩⟩ := WBisim'.stepVis h' h.symm
+    have h := h.toEStep.transp_bind_map k1
+    have h' := h'.toEStep.transp_bind_map k1
+    refine .vis (Classical.choice h.toVisStep) (Classical.choice h'.toVisStep) ?_
+    intro v
+    simp only [Function.comp_apply, dest_bind]
+    refine ⟨_, _, bs v, rfl, rfl⟩
+
+theorem bind_congr_cont
+    {X} {k1 k2 : KTree E A X}
+    (h : k1 ≈ₖ k2)
+    : bind a k1 ≈ bind a k2 := by
+  simp [WBisim]
+  refine ⟨
+    fun a b => WBisim' E X a b ∨ ∃ k1 k2 v, k1 ≈ₖ k2
+        ∧ bind_map k1 v = a
+        ∧ bind_map k2 v = b,
+    ?_,
+    .inr ⟨_,_, _, h, rfl, rfl⟩
+  ⟩
+  rintro a b (h|⟨k1, k2, w, h, rfl, rfl⟩)
+  · exact match h.unfold with
+    | .refl ha hb => .refl ha hb
+    | .ret ha hb => .ret ha hb
+    | .vis ha hb h => .vis ha hb (.inl <| h ·)
+  rcases Step.no_middle w with (rfl|⟨⟨w,⟨h'⟩⟩⟩|⟨⟨_,_,_,⟨h'⟩⟩⟩)
+  · simp only [bind_map.tau, spin.bind_eq]
+    exact .refl'
+  all_goals
+    apply WBisim'.Invariant.skip
+      (h'.toEStep.transp_bind_map k1)
+      (h'.toEStep.transp_bind_map k2)
+  all_goals dsimp
+  · specialize h w
+    exact match h.unfold with
+    | .refl ha hb => .refl ha hb
+    | .ret ha hb => .ret ha hb
+    | .vis ha hb h => .vis ha hb (.inl <| h ·)
+
+  · refine .vis .vis .vis fun w => .inr ?_
+    simp only [Function.comp_apply, dest_bind]
+    exact ⟨_,_,_, h, rfl, rfl⟩
+
+theorem bind_congr {X} {k1 k2 : KTree E A X}
+    (h : a ≈ b)
+    (h' : k1 ≈ₖ k2)
+    : bind a k1 ≈ bind b k2 := calc
+  bind a k1
+    ≈ bind a k2 := bind_congr_cont h'
+  _ ≈ bind b k2 := bind_congr_arg h
+
+theorem iter_bisim {it : A → ITree E (A ⊕ B)} {v}
+    : iter it v ≈ (it v).bind (Sum.elim (iter it) ITree.ret) := by
+  rw [iter_eq]
+  exact bind_congr_cont fun | .inr _ => .refl | .inl _ => tau
+
+end ITree.WBisim
+
+end Sme
 
