sme/Sme/ITree/KTree.lean
@@ -1,0 +1,23 @@
+import CoinductivePredicates
+import Sme.ITree.Defs
+import Sme.ITree.Combinators
+
+namespace Sme
+
+universe u v
+
+variable {E : Type u → Type u} {A B C : Type _}
+
+def KTree (E : Type u → Type u) (A B : Type _) : Type _ := A → ITree E B
+
+namespace KTree
+
+open ITree
+
+def id (A : Type _) : KTree E A A := .ret
+def comp (a : KTree E A B) (b : KTree E B C) : KTree E A C := subst b ∘ a
+
+end KTree
+
+end Sme
+
